give 1/2 serv gs to iris inv so that clients can learn freshness w/o selfmon. specify all the ghost and physical invs in own_serv

src/program_proof/pav/server.v
@@ -25,7 +25,7 @@ End userState.
 Module servEpochInfo.
 Record t :=
   mk {
-    updates: gmap byte_string (list w8);
+    updates: gmap (list w8) (w64 * list w8);
     dig: list w8;
     sig: list w8;
   }.
@@ -35,8 +35,9 @@ Context `{!heapGS Σ, !pavG Σ}.
 
 Definition own ptr x : iProp Σ :=
   ∃ ptr2_upd ptr_upd sl_dig sl_sig,
-  "#Hupd" ∷ ([∗ map] sl;u ∈ ptr2_upd;x.(updates),
-    own_slice_small sl byteT DfracDiscarded u) ∗
+  "#Hupd" ∷ ([∗ map] sl;y ∈ ptr2_upd;x.(updates),
+    own_slice_small sl byteT DfracDiscarded
+      (MapValPre.encodesF $ MapValPre.mk y.1 y.2)) ∗
   "#Hptr2_upd" ∷ own_map ptr_upd DfracDiscarded ptr2_upd ∗
   "#Hptr_upd" ∷ ptr ↦[servEpochInfo :: "updates"]□ #ptr_upd ∗
   "#Hsl_dig" ∷ own_slice_small sl_dig byteT DfracDiscarded x.(dig) ∗
@@ -52,8 +53,8 @@ Record t :=
     sig_pk: list w8;
     vrf_pk: list w8;
     γepoch: gname;
-    γdigs: gname;
-    γmap: gname;
+    γsig: gname;
+    γcli: gname;
   }.
 End Server.
 
@@ -66,40 +67,111 @@ Definition serv_sigpred (γ : gname) : (list w8 → iProp Σ) :=
 
 Definition is_WorkQ (ptr : loc) : iProp Σ. Admitted.
 
-Definition own_Server (ptr : loc) (d : dfrac) : iProp Σ :=
+Definition maps_mono (ms : list adtr_map_ty) :=
+  ∀ (i j : w64) mi mj,
+  ms !! (uint.nat i) = Some mi →
+  ms !! (uint.nat j) = Some mj →
+  uint.Z i ≤ uint.Z j →
+  mi ⊆ mj.
+
+Definition epochs_ok (ms : list adtr_map_ty) :=
+  ∀ (ep : w64) m_ep k ep' comm,
+  ms !! (uint.nat ep) = Some m_ep →
+  m_ep !! k = Some (ep', comm) →
+  uint.Z ep' ≤ uint.Z ep.
+
+Definition lower_map (m : adtr_map_ty) : merkle_map_ty :=
+  (λ v, MapValPre.encodesF (MapValPre.mk v.1 v.2)) <$> m.
+
+(* inv_gs will be a proper iris invariant so that clients can access
+and learn that their own key is fresh even in latest epoch. *)
+Definition inv_gs serv : iProp Σ :=
+  ∃ gs_hist gs_vers,
+  "Hgs_ep" ∷ mono_nat_auth_own serv.(Server.γepoch) (1/2) (length gs_hist) ∗
+  "Hgs_sig" ∷ mono_list_auth_own serv.(Server.γsig) (1/2) gs_hist ∗
+  "Hgs_cli" ∷ ghost_map_auth serv.(Server.γcli) (1/2) gs_vers ∗
+
+  "%Hmono_maps" ∷ ⌜ maps_mono gs_hist.*1 ⌝ ∗
+  "%Hok_epochs" ∷ ⌜ epochs_ok gs_hist.*1 ⌝ ∗
+  "#Hok_vers" ∷ ([∗ map] uid ↦ nVers ∈ gs_vers,
+    ∃ label,
+    "#Hvrf_out" ∷ is_vrf_out serv.(Server.vrf_pk)
+      (MapLabelPre.encodesF $ MapLabelPre.mk uid nVers) label ∗
+    "%Hlook_map" ∷ ⌜ (default ∅ (last gs_hist.*1)) !! label = None ⌝).
+
+Definition own_Server ptr serv q : iProp Σ :=
   ∃ ptr_key_map key_map ptr_user_info
-    (ptr2_user_info : gmap w64 _) user_info
-    sl_epoch_hist ptr2_epoch_hist epoch_hist,
-  "HkeyM" ∷ own_Tree ptr_key_map key_map d ∗
+    ptr2_user_info user_info sl_commit_secret commit_secret
+    sl_epoch_hist ptr2_epoch_hist epoch_hist
+    gs_hist gs_vers,
+
+  (* ghost ownership. the other 1/2 is in the invariant. *)
+  "Hgs_ep" ∷ mono_nat_auth_own serv.(Server.γepoch) (1/2) (length gs_hist) ∗
+  "Hgs_sig" ∷ mono_list_auth_own serv.(Server.γsig) (1/2) gs_hist ∗
+  "Hgs_cli" ∷ ghost_map_auth serv.(Server.γcli) (1/2) gs_vers ∗
+
+  (* physical ownership. *)
+  "HkeyM" ∷ own_Tree ptr_key_map key_map (DfracOwn q) ∗
   "#Hptr_keyM" ∷ ptr ↦[Server :: "keyMap"]□ #ptr_key_map ∗
-  "Huinfo" ∷ ([∗ map] l;x ∈ ptr2_user_info;user_info, userState.own l x d) ∗
-  "Hptr2_uinfo" ∷ own_map ptr_user_info d ptr2_user_info ∗
+  "Huinfo" ∷ ([∗ map] l;x ∈ ptr2_user_info;user_info,
+    userState.own l x (DfracOwn q)) ∗
+  "Hptr2_uinfo" ∷ own_map ptr_user_info (DfracOwn q) ptr2_user_info ∗
   "#Hptr_uinfo" ∷ ptr ↦[Server :: "userInfo"]□ #ptr_user_info ∗
-  "#Hep_hist" ∷ ([∗ list] l;x ∈ ptr2_epoch_hist;epoch_hist, servEpochInfo.own l x) ∗
-  "Hptr2_ep_hist" ∷ own_slice sl_epoch_hist ptrT d ptr2_epoch_hist ∗
-  "Hptr_ep_hist" ∷ ptr ↦[Server :: "epochHist"]{d} (slice_val sl_epoch_hist).
+  "#Hep_hist" ∷ ([∗ list] l;x ∈ ptr2_epoch_hist;epoch_hist,
+    servEpochInfo.own l x) ∗
+  "Hptr2_ep_hist" ∷ own_slice sl_epoch_hist ptrT (DfracOwn q) ptr2_epoch_hist ∗
+  "Hptr_ep_hist" ∷ ptr ↦[Server :: "epochHist"]{DfracOwn q} (slice_val sl_epoch_hist) ∗
+  "#Hsl_sec" ∷ own_slice_small sl_commit_secret byteT DfracDiscarded commit_secret ∗
+  "#Hptr_sec" ∷ ptr ↦[Server :: "commitSecret"]□ (slice_val sl_commit_secret) ∗
+
+  (* physical invariants. *)
+  "#Hsig_hist" ∷ ([∗ list] ep ↦ x ∈ epoch_hist,
+    is_sig serv.(Server.sig_pk)
+      (PreSigDig.encodesF $ PreSigDig.mk (W64 ep) x.(servEpochInfo.dig))
+      x.(servEpochInfo.sig)) ∗
+  "Hplain_pk" ∷ ([∗ map] uid ↦ x ∈ user_info,
+    ∃ label commit ep,
+    "#Hvrf_out" ∷ is_vrf_out serv.(Server.vrf_pk)
+      (MapLabelPre.encodesF $
+        MapLabelPre.mk uid (word.sub x.(userState.numVers) (W64 1)))
+      label ∗
+    "#Hcommit" ∷ is_hash (CommitOpen.encodesF $
+      CommitOpen.mk x.(userState.plainPk) commit_secret)
+      commit ∗
+    "%Hlook_map" ∷ ⌜ key_map !! label =
+      Some (MapValPre.encodesF $ MapValPre.mk ep commit) ⌝) ∗
+
+  (* physical-ghost reln. *)
+  "%Heq_dig_hist" ∷ ⌜ gs_hist.*2 = servEpochInfo.dig <$> epoch_hist ⌝ ∗
+  "%Heq_vers" ∷ ⌜ gs_vers = userState.numVers <$> user_info ⌝ ∗
+  "%Heq_keyM" ∷ ⌜ key_map = lower_map (default ∅ (last gs_hist.*1)) ⌝ ∗
+  "%Heq_map_hist" ∷ ([∗ list] ep ↦ x ∈ (drop 1 epoch_hist),
+    ∃ prevM nextM,
+    "%Hlook_prevM" ∷ ⌜ gs_hist.*1 !! (pred ep) = Some prevM ⌝ ∗
+    "%Hlook_nextM" ∷ ⌜ gs_hist.*1 !! ep = Some nextM ⌝ ∗
+    "%Hupd" ∷ ⌜ nextM = x.(servEpochInfo.updates) ∪ prevM ⌝).
 
 Definition is_Server ptr serv : iProp Σ :=
-  ∃ mu ptr_sig_sk sig_pk γ ptr_vrf_sk
-    sl_commit_secret (commit_secret : list w8) ptr_workq,
-  "#HmuR" ∷ is_rwlock nroot #mu (λ q, own_Server ptr (DfracOwn (q / 2))) ∗
+  ∃ mu ptr_sig_sk sig_pk γ ptr_vrf_sk ptr_workq,
+  "#Hinv_gs" ∷ inv nroot (inv_gs serv) ∗
+  "#HmuR" ∷ is_rwlock nroot #mu (λ q, own_Server ptr serv (q / 2)) ∗
   "#Hptr_mu" ∷ ptr ↦[Server :: "mu"]□ #mu ∗
   "#Hsig_sk" ∷ is_sig_sk ptr_sig_sk sig_pk (serv_sigpred γ) ∗
   "#Hptr_sig_sk" ∷ ptr ↦[Server :: "sigSk"]□ #ptr_sig_sk ∗
   "#Hvrf_sk" ∷ is_vrf_sk ptr_vrf_sk serv.(Server.vrf_pk) ∗
   "#Hptr_vrf_sk" ∷ ptr ↦[Server :: "vrfSk"]□ #ptr_vrf_sk ∗
-  "#Hsl_sec" ∷ own_slice_small sl_commit_secret byteT DfracDiscarded commit_secret ∗
-  "#Hptr_sec" ∷ ptr ↦[Server :: "commitSecret"]□ (slice_val sl_commit_secret) ∗
   "#Hworkq" ∷ is_WorkQ ptr_workq ∗
   "#Hptr_workq" ∷ ptr ↦[Server :: "workQ"]□ #ptr_workq.
 
 Definition wish_memb vrf_pk uid ver sigdig memb : iProp Σ :=
-  ∃ label map_val,
+  ∃ label commit,
   let label_pre := (MapLabelPre.encodesF $ MapLabelPre.mk uid ver) in
   "#Hvrf_proof" ∷ is_vrf_proof vrf_pk label_pre memb.(Memb.LabelProof) ∗
   "#Hvrf_out" ∷ is_vrf_out vrf_pk label_pre label ∗
-  "#Hmap_val" ∷ is_hash (CommitOpen.encodesF memb.(Memb.PkOpen)) map_val ∗
-  "#Hmerk" ∷ Verify_wish true label map_val memb.(Memb.MerkleProof) sigdig.(SigDig.Dig).
+  "#Hcommit" ∷ is_hash (CommitOpen.encodesF memb.(Memb.PkOpen)) commit ∗
+  "#Hmerk" ∷ Verify_wish true label
+    (MapValPre.encodesF $ MapValPre.mk sigdig.(SigDig.Epoch) commit)
+    memb.(Memb.MerkleProof) sigdig.(SigDig.Dig).
 
 Definition wish_nonmemb vrf_pk uid ver sigdig nonmemb : iProp Σ :=
   ∃ label,
@@ -109,17 +181,10 @@ Definition wish_nonmemb vrf_pk uid ver sigdig nonmemb : iProp Σ :=
   "#Hmerk" ∷ Verify_wish false label [] nonmemb.(NonMemb.MerkleProof)
     sigdig.(SigDig.Dig).
 
-(* TODO: server correctness not just that all client fns
-(including audit) will not error.
-also that without even talking to auditor, clients can have agreement.
-for that, the server needs to guarantee that put / get elems
-are actually in server ghost state, and that ghost state
-satisfies certain invs, similar to auditor. *)
-
 Lemma wp_Server__Put ptr serv uid nVers sl_pk (pk : list w8) cli_ep :
   {{{
     "#Hserv" ∷ is_Server ptr serv ∗
-    "Hpks" ∷ uid ↪[serv.(Server.γmap)] nVers ∗
+    "Hpks" ∷ uid ↪[serv.(Server.γcli)] nVers ∗
     "#Hsl_pk" ∷ own_slice_small sl_pk byteT DfracDiscarded pk ∗
     "#Hlb_ep" ∷ mono_nat_lb_own serv.(Server.γepoch) cli_ep
   }}}
@@ -127,7 +192,7 @@ Lemma wp_Server__Put ptr serv uid nVers sl_pk (pk : list w8) cli_ep :
   {{{
     ptr_sigdig sigdig ptr_memb memb ptr_nonmemb nonmemb err,
     RET (#ptr_sigdig, #ptr_memb, #ptr_nonmemb, #err);
-    "Hpks" ∷ uid ↪[serv.(Server.γmap)] (nVers + 1) ∗
+    "Hpks" ∷ uid ↪[serv.(Server.γcli)] (word.add nVers (W64 1)) ∗
     "%Heq_ep" ∷ ⌜ sigdig.(SigDig.Epoch) = memb.(Memb.EpochAdded) ⌝ ∗
     "%Heq_pk" ∷ ⌜ pk = memb.(Memb.PkOpen).(CommitOpen.Val) ⌝ ∗
     "#Hsigdig" ∷ SigDig.own ptr_sigdig sigdig DfracDiscarded ∗
@@ -139,10 +204,10 @@ Lemma wp_Server__Put ptr serv uid nVers sl_pk (pk : list w8) cli_ep :
     "#Hlb_ep" ∷ mono_nat_lb_own serv.(Server.γepoch) (uint.nat sigdig.(SigDig.Epoch)) ∗
     "%Hlt_ep" ∷ ⌜ Z.of_nat cli_ep < uint.Z sigdig.(SigDig.Epoch) ⌝ ∗
     "Hmemb" ∷ Memb.own ptr_memb memb (DfracOwn 1) ∗
-    "#Hwish_memb" ∷ wish_memb serv.(Server.vrf_pk) uid (W64 $ nVers) sigdig memb ∗
+    "#Hwish_memb" ∷ wish_memb serv.(Server.vrf_pk) uid nVers sigdig memb ∗
     "Hnonmemb" ∷ NonMemb.own ptr_nonmemb nonmemb (DfracOwn 1) ∗
     "#Hwish_nonmemb" ∷ wish_nonmemb serv.(Server.vrf_pk)
-      uid (W64 $ (nVers + 1)) sigdig nonmemb ∗
+      uid (word.add nVers (W64 1)) sigdig nonmemb ∗
     "%Herr" ∷ ⌜ err = false ⌝
   }}}.
 Proof. Admitted.
